git rid of mtdc, added roots

Cheriot/Config.v
@@ -197,33 +197,25 @@ Section CapHelpers.
       getCapBounds ty base length := capBounds base length;
     |}%kami_expr.
 
-  Definition PcCapInit := evalExpr (@pack _ CapStruct
-                                      (STRUCT {
-                                           "R" ::= Const _ (wzero _);
-                                           "p" ::= Const _ ('b"101111");
-                                           "oType" ::= Const _ (wzero _);
-                                           "E" ::= Const _ (wones _);
-                                           "B" ::= Const _ (wzero _);
-                                           "T" ::= Const _ (_ 'h"100") })%kami_expr).
+  Definition ExecRootCapInit := evalExpr (@pack _ CapStruct
+                                            (STRUCT {
+                                                 "R" ::= Const _ (wzero _);
+                                                 "p" ::= Const _ ('b"101111");
+                                                 "oType" ::= Const _ (wzero _);
+                                                 "E" ::= Const _ (wones _);
+                                                 "B" ::= Const _ (wzero _);
+                                                 "T" ::= Const _ (_ 'h"100") })%kami_expr).
 
-  Definition PcAddrInit := (AddrSz 'h"1000").
+  Definition DataRootCapInit := evalExpr (@pack _ CapStruct
+                                            ( STRUCT {
+                                                  "R" ::= Const _ (wzero _);
+                                                  "p" ::= Const _ ('b"111111");
+                                                  "oType" ::= Const _ (wzero _);
+                                                  "E" ::= Const _ (wones _);
+                                                  "B" ::= Const _ (wzero _);
+                                                  "T" ::= Const _ (_ 'h"100") })%kami_expr).
 
-  Definition MtccCapInit := PcCapInit.
-
-  Definition MtccValInit := (AddrSz 'h"800").
-
-  Definition MtdcCapInit := evalExpr (@pack _ CapStruct
-                                        ( STRUCT {
-                                              "R" ::= Const _ (wzero _);
-                                              "p" ::= Const _ ('b"111111");
-                                              "oType" ::= Const _ (wzero _);
-                                              "E" ::= Const _ (wones _);
-                                              "B" ::= Const _ (wzero _);
-                                              "T" ::= Const _ (_ 'h"100") })%kami_expr).
-  
-  Definition MtdcValInit := (AddrSz 'h"400").
-
-  Definition MScratchCapInit := evalExpr (@pack _ CapStruct
+  Definition SealRootCapInit := evalExpr (@pack _ CapStruct
                                             (STRUCT {
                                                  "R" ::= Const _ (wzero _);
                                                  "p" ::= Const _ ('b"100111");
@@ -232,9 +224,11 @@ Section CapHelpers.
                                                  "B" ::= Const _ (wzero _);
                                                  "T" ::= Const _ (_ 'h"100") })%kami_expr).
 
-  Definition MScratchValInit := (AddrSz 'h"0").
+  Definition PcAddrInit := (AddrSz 'h"1000").
+  Definition MtccValInit := (AddrSz 'h"800").
+  Definition MtdcValInit := (AddrSz 'h"400").
 
-  Theorem pccValidThm: PccValid capAccessorsInit PcCapInit PcAddrInit false.
+  Theorem pccValidThm: PccValid capAccessorsInit ExecRootCapInit PcAddrInit false.
   Proof.
     repeat constructor; auto.
   Qed.
@@ -257,12 +251,10 @@ Section Prefix.
       xlenIs32_or_64 := or_introl eq_refl;
       capAccessors := capAccessorsInit;
       pccValid := pccValidThm;
-      MtccCap := MtccCapInit;
+      ExecRootCap := ExecRootCapInit;
+      DataRootCap := DataRootCapInit;
+      SealRootCap := SealRootCapInit;
       MtccVal := MtccValInit;
-      MtdcCap := MtdcCapInit;
-      MtdcVal := MtdcValInit;
-      MScratchCap := MScratchCapInit;
-      MScratchVal := MScratchValInit;
       IeInit := false;
       MeieInit := false;
       MtieInit := false;
